src/Checker.v
@@ -21,7 +21,7 @@ Inductive CallbackKind :=
 
 Inductive SmallResult :=
   MkSmallResult : option bool -> bool -> string -> bool ->
-                  list (string * nat) -> SmallResult.
+                  list string -> SmallResult.
 
 Inductive Callback : Type :=
 | PostTest :
@@ -31,12 +31,12 @@ Inductive Callback : Type :=
 
 Record Result :=
   MkResult {
-      ok : option bool;
-      expect : bool;
-      reason : string;
-      interrupted : bool;
-      stamp : list (string * nat);
-      callbacks : list Callback
+      ok          : option bool; (* Test case result - maybe == discard *)
+      expect      : bool;        (* If false, property should fail *)
+      reason      : string;      (* Error message *)
+      interrupted : bool;        (* ? *)
+      stamp       : list string; (* Collected values for this test case *)
+      callbacks   : list Callback
     }.
 
 (* I WANT RECORD UPDATES :'( *)
@@ -112,6 +112,10 @@ Global Instance testGenProp (P : Type) : Checkable P -> Checkable (G P) :=
     checker p := bindGen p checker
   |}.
 
+Global Instance testChecker : Checkable Checker :=
+  {| 
+      checker x := x 
+  |}.
 
 (* Checker Combinators *)
 
@@ -159,12 +163,13 @@ Definition expectFailure {prop: Type} `{Checkable prop} (p: prop) :=
                              (interrupted res) (stamp res) (callbacks res))
                  p.
 
+(* NOTE: Ignoring the nat argument. Use label or collect ONLY *)
 Definition cover {prop : Type} {_ : Checkable prop}
            (b : bool) (n : nat) (s : string) : prop -> Checker :=
   if b then
     mapTotalResult (fun res =>
                       let '(MkResult o e r i st c) := res in
-                      MkResult o e r i ((s,n)::st) c)
+                      MkResult o e r i (s :: st) c)
   else checker.
 
 Definition classify {prop : Type} {_ : Checkable prop}
