src/State.v
@@ -4,6 +4,11 @@ Require Import ModuleGen.
 Require Import Axioms.
 Require Import String.
 
+Require Import StringOT.
+Require Import FSets.FMapAVL.
+
+Module Map := FMapAVL.Make(StringOT).
+
 Record State := MkState
   { maxSuccessTests   : nat
   ; maxDiscardedTests : nat
@@ -12,7 +17,9 @@ Record State := MkState
 
   ; numSuccessTests   : nat
   ; numDiscardedTests : nat
-  ; collected         : list (list (string * nat))
+
+  ; labels            : Map.t nat
+
   ; expectedFailure   : bool
   ; randomSeed        : RandomGen
 
@@ -22,12 +29,12 @@ Record State := MkState
 
 Definition updTryShrinks (st : State) (f : nat -> nat) : State :=
   match st with
-    | MkState mst mdt ms cs nst ndt c e r nss nts =>
-      MkState mst mdt ms cs nst ndt c e r nss (f nts)
+    | MkState mst mdt ms cs nst ndt ls e r nss nts =>
+      MkState mst mdt ms cs nst ndt ls e r nss (f nts)
   end.
 
 Definition updSuccessShrinks (st : State) (f : nat -> nat) : State :=
   match st with
-    | MkState mst mdt ms cs nst ndt c e r nss nts =>
-      MkState mst mdt ms cs nst ndt c e r (f nss) nts
+    | MkState mst mdt ms cs nst ndt ls e r nss nts =>
+      MkState mst mdt ms cs nst ndt ls e r (f nss) nts
   end.
